Isa/Exp.v
@@ -19,7 +19,9 @@ Set Implicit Arguments.
       | 2 => option_lift2 bvMult
       | 3 => option_lift2 bvEq
       | 4 => option_lift2 (fun a b => neg (bvEq a b))
-      | _ => bvDiv
+      | 5 => bvDiv
+      | _ => option_lift2 (fun a b => sext k nil O)
+(*      | _ => option_lift2 bvAdd (*fun _ _ => None *) *)
     end.
 
   Definition unop : Set := nat.
