TransVal/GuardProps.v
@@ -4,6 +4,8 @@ Require Import SetOperations Sim Var.
 Require Import smt nofun noGoto bitvec freeVars.
 Require Import Compute Guards ILFtoSMT tvalTactics TUtil.
 
+Opaque zext.
+
 (* TODO Move *)
 Lemma exp_freeVars_list_agree (E: onv val) e el:
     (forall x, x ∈ list_union (Exp.freeVars e:: List.map Exp.freeVars el) -> exists v, E x = Some v)
@@ -18,633 +20,163 @@ Proof.
     cset_tac; eauto.
 Qed.
 
+
+Lemma exp_freeVars_bin_agree (E:onv val) a b:
+  (forall x, x ∈ (Exp.freeVars a ++ Exp.freeVars b) -> exists v, E x = Some v)
+    ->(forall x, x ∈ Exp.freeVars a -> (exists v, E x = Some v)) /\
+      (forall x, x ∈ Exp.freeVars b -> exists v, E x = Some v).
+
+Proof.
+  intros.
+  split; intros; specialize (H x); destruct H; cset_tac; eauto.
+Qed.
+
 (** Lemma 5 in the thesis.
 Proves that whenever an expression evaluates under
 a partial environment, then it's guard must be satisfiable **)
  Lemma guard_true_if_eval:
-forall F E e s v,
+forall F E e v,
  exp_eval E e = Some v
-->  undef e = Some s
-->  models F (to_total E) s.
+->  models F (to_total E) (undef e).
 
 Proof.
-intros. general induction e; simpl.
-- simpl in *. monad_inv H. destruct u.
-  + apply (IHe F E s x); eauto.
-  +  apply (IHe F E s x); eauto.
-- simpl in H.  monad_inv H.  simpl in H0. destruct b.
-  +  case_eq (undef e1); case_eq (undef e2); intros.
-     *  rewrite H in H0; rewrite H1 in H0. simpl in H0.
-        inversion H0. simpl; split.
-        { eapply IHe1; eauto. }
-        { eapply IHe2; eauto. }
-     * rewrite H in H0; rewrite H1 in H0; simpl in H0; inversion H0; simpl.
-       eapply IHe1; eauto. rewrite <- H0; eauto.
-     * rewrite H in H0; rewrite H1 in H0; simpl in H0; inversion H0; simpl.
-       eapply IHe2; eauto. rewrite <- H0; eauto.
-     * rewrite H in H0; rewrite H1 in H0; simpl in H0;  simpl.
-       exfalso; discriminate H0.
-  + destruct b.
-    *  case_eq (undef e1); case_eq (undef e2); intros.
-     {  rewrite H in H0; rewrite H1 in H0. simpl in H0. inversion H0.
-        simpl; split.
-        - eapply IHe1; eauto.
-        - eapply IHe2; eauto. }
-     { rewrite H in H0; rewrite H1 in H0; simpl in H0; inversion H0; simpl.
-       eapply IHe1; eauto. rewrite <- H0; eauto. }
-     { rewrite H in H0; rewrite H1 in H0; simpl in H0; inversion H0; simpl.
-       eapply IHe2; eauto. rewrite <- H0; eauto. }
-     { rewrite H in H0; rewrite H1 in H0; simpl in H0;  simpl.
-       exfalso; discriminate H0. }
-    * destruct b.
-      { case_eq (undef e1); case_eq (undef e2); intros.
-        -  rewrite H in H0; rewrite H1 in H0. simpl in H0. inversion H0.
-simpl; split.
-           + eapply IHe1; eauto.
-           + eapply IHe2; eauto.
-        - rewrite H in H0; rewrite H1 in H0; simpl in H0; inversion H0; simpl.
-          eapply IHe1; eauto. rewrite <- H0; eauto.
-        - rewrite H in H0; rewrite H1 in H0; simpl in H0; inversion H0; simpl.
-          eapply IHe2; eauto. rewrite <- H0; eauto.
-        - rewrite H in H0; rewrite H1 in H0; simpl in H0;  simpl.
-          exfalso; discriminate H0. }
-      { destruct b.
-        -  case_eq (undef e1); case_eq (undef e2); intros.
-           +  rewrite H in H0; rewrite H1 in H0. simpl in H0. inversion H0.
-              simpl; split.
-              * eapply IHe1; eauto.
-              * eapply IHe2; eauto.
-           + rewrite H in H0; rewrite H1 in H0; simpl in H0; inversion H0.
-             simpl. eapply IHe1; eauto. rewrite <- H0; eauto.
-           + rewrite H in H0; rewrite H1 in H0; simpl in H0; inversion H0.
-             simpl. eapply IHe2; eauto. rewrite <- H0; eauto.
-            +rewrite H in H0; rewrite H1 in H0; simpl in H0;  simpl.
-             exfalso; discriminate H0.
-        - destruct b.
-          +  case_eq (undef e1); case_eq (undef e2); intros.
-             *  rewrite H in H0; rewrite H1 in H0. simpl in H0. inversion H0.
-                simpl; split.
-                { eapply IHe1; eauto. }
-                { eapply IHe2; eauto. }
-             * rewrite H in H0; rewrite H1 in H0; simpl in H0; inversion H0.
-               simpl. eapply IHe1; eauto. rewrite <- H0; eauto.
-             *rewrite H in H0; rewrite H1 in H0; simpl in H0; inversion H0.
-              simpl. eapply IHe2; eauto. rewrite <- H0; eauto.
-             * rewrite H in H0; rewrite H1 in H0; simpl in H0;  simpl.
-               exfalso; discriminate H0.
-          + simpl in EQ2.
-            * case_eq (undef e1); case_eq (undef e2); intros.
-              {  rewrite H in H0; rewrite H1 in H0. simpl in H0. inversion H0.
-                 unfold binop_eval in EQ2.  clear H0. unfold bvDiv in EQ2.
-                 simpl. split.
-                 - case_eq(bvZero x0).
-                   + intros.  rewrite H0 in EQ2.  exfalso; discriminate EQ2.
-                   + intros A.   intros. clear H3. clear EQ2.
-                     hnf in H0. unfold smt_eval in H0.
-                     erewrite exp_eval_partial_total in H0; eauto.
-                     simpl in H0. simpl  in A.
-                     eapply  (not_zero_implies_uneq _  A) in H0;  eauto.
-                 - split.
-                   + eapply IHe1; eauto.
-                   + eapply IHe2; eauto.  }
-                 { rewrite H in H0; rewrite H1 in H0; simpl in H0. inversion H0.
-                   unfold binop_eval in EQ2. clear H0. unfold bvDiv in EQ2.
-                   simpl. split.
-                 - case_eq(bvZero x0).
-                   + intros.  rewrite H0 in EQ2.  exfalso; discriminate EQ2.
-                   + intros A.   intros. clear H3. clear EQ2.
-                     hnf in H0.
-                     unfold smt_eval in H0;
-                       erewrite exp_eval_partial_total in H0; eauto.
-                     simpl in H0. simpl  in A.
-                     eapply ( not_zero_implies_uneq _) in H0; eauto.
-                 -  eapply IHe1; eauto. }
-                 { rewrite H in H0; rewrite H1 in H0; simpl in H0. inversion H0.
-                   unfold binop_eval in EQ2. clear H0. unfold bvDiv in EQ2.
-                   simpl. split.
-                 - case_eq(bvZero x0).
-                   + intros.  rewrite H0 in EQ2.  exfalso; discriminate EQ2.
-                   + intros A.  intros. clear H3. clear EQ2.
-                     hnf in H0.
-                     unfold smt_eval in *;
-                       erewrite exp_eval_partial_total in H0; eauto.
-                     simpl in H0. simpl  in A.
-                     eapply  (not_zero_implies_uneq _) in H0; eauto.
-                 -  eapply IHe2; eauto. }
-                 { rewrite H in H0; rewrite H1 in H0; simpl in H0. inversion H0.
-                   unfold binop_eval in EQ2. clear H0.
-                   unfold bvDiv in EQ2. simpl.
-                   case_eq(bvZero x0).
-                   - intros.  rewrite H0 in EQ2.  exfalso; discriminate EQ2.
-                   - intros A. intros. clear H3. clear EQ2.
-                     hnf in H0.
-                     unfold smt_eval in *;
-                     erewrite exp_eval_partial_total in H0; eauto.
-                     simpl in H0. simpl  in A.
-                     eapply  (not_zero_implies_uneq _ ) in H0; eauto. } }
+intros. general induction e; simpl in *; eauto.
+- monad_inv H.
+  eapply IHe; eauto.
+- monad_inv H.
+  destruct if.
+   + erewrite models_combine; simpl; erewrite models_combine; simpl.
+     split; try split; eauto.
+     intros.
+     unfold val2bool in H.
+     eapply bvEq_equiv_eq in H.
+     unfold smt_eval in H.
+     erewrite exp_eval_partial_total in H; eauto.
+     simpl in H.
+     rewrite H in EQ2; subst; simpl in EQ2; isabsurd.
+   + erewrite models_combine; simpl; erewrite models_combine; simpl.
+     split; try split; eauto.
 Qed.
 
 (** Lemma 5 in the thesis, lifted to lists **)
 Lemma guardList_true_if_eval:
-forall F E el s vl,
+forall F E el vl,
 omap (exp_eval E) el = Some vl
--> undefLift el = Some s
--> models F (to_total E) s.
+-> models F (to_total E) (undefLift el).
 
 Proof.
-intros. general induction el.
-- simpl in *.  case_eq (undef a); intros.
-  + rewrite H1 in H0. simpl in H0.  case_eq (undefLift el); intros; simpl.
-    * rewrite H2 in H0. inversion H0. simpl. split.
-      { monad_inv H. eapply (guard_true_if_eval); eauto. }
-      { monad_inv H. eapply IHel; eauto. }
-    * rewrite H2 in H0. inversion H0. monad_inv H.
-      eapply (guard_true_if_eval); eauto.
-  + rewrite H1 in H0; monad_inv H. eapply IHel; eauto.
+intros. general induction el; simpl in *; eauto.
+monad_inv H.
+erewrite models_combine; simpl; split; eauto using guard_true_if_eval.
 Qed.
 
-(** Not in thesis due to simplification fo guards as booleans without
-options
---> approx. Lema 6 **)
-Lemma noguard_impl_eval:
-forall E e,
+(** Lemma 6 **)
+Lemma guard_models_impl_eval:
+forall F E e,
 (forall x, x ∈ Exp.freeVars e -> exists v,  E x = Some v)
--> undef e = None
+-> models F (to_total E) (undef e)
 -> exists v, exp_eval E e = Some v.
 
 Proof.
-  intros. general induction e.
-  - exists v. unfold exp_eval. reflexivity.
-  - destruct (H v); simpl; cset_tac; eauto.
-  - simpl in H. specialize (IHe E H). simpl in H0.
-     destruct IHe; eauto.
-     simpl. rewrite H1. simpl. destruct u; simpl.
+  intros. general induction e; simpl in *; eauto.
+  - destruct (H v); cset_tac; eauto.
+  - destruct (IHe F E); subst; destruct u; eauto; simpl; rewrite H1.
     + case_eq (val2bool x); intros.
-      * exists val_true; unfold option_lift1; simpl.
-          rewrite H2; eauto.
-      * exists val_false; unfold option_lift1; simpl.
-         rewrite H2; eauto.
-      + exists (neg x); unfold option_lift1.
-          destruct u; eauto.
-  - specialize (IHe1 E); specialize (IHe2 E). simpl in H. cset_tac.
-    assert (forall x, x ∈ Exp.freeVars e1 -> exists v, E x = Some v)
-      by (cset_tac; eauto).
-    assert (forall x, x ∈ Exp.freeVars e2 -> exists v, E x  = Some v)
-      by (cset_tac; eauto).
-    specialize (IHe1 H1); specialize (IHe2 H2).
-    destructBin b; simpl in *.
-    + eapply combine_keep_undef in H0. destruct H0.
-      destruct IHe1; destruct IHe2; eauto.
-      rewrite H4; rewrite H5. simpl. exists (bvAdd x x0).
-      unfold option_lift2; eauto.
-    + eapply combine_keep_undef in H0; destruct H0.
-      destruct IHe1, IHe2; eauto.
-      rewrite H4; rewrite H5; simpl; exists (bvSub x x0).
-      unfold option_lift2; eauto.
-    + eapply combine_keep_undef in H0; destruct H0.
-      destruct IHe1, IHe2; eauto.
-      rewrite H4, H5; simpl; exists (bvMult x x0).
-      unfold option_lift2; eauto.
-    + eapply combine_keep_undef in H0; destruct H0.
-      destruct IHe1, IHe2; eauto.
-      rewrite H4, H5; simpl; exists (bvEq x x0).
-      unfold option_lift2; eauto.
-    + eapply combine_keep_undef in H0; destruct H0.
-      destruct IHe1, IHe2; eauto.
-      rewrite H4, H5; simpl; exists (neg (bvEq x x0)).
-      unfold option_lift2; eauto.
-    + case_eq (undef e1); case_eq(undef e2); intros;
-      rewrite H3 in *; rewrite H4 in *; discriminate H0.
+      * exists val_true; simpl; unfold option_lift1; rewrite H2; simpl; eauto.
+      * exists val_false; simpl; unfold option_lift1; rewrite H2; simpl; eauto.
+    + exists (neg x). simpl; unfold option_lift1; eauto.
+  - simpl in *.
+    repeat (rewrite models_combine in H0; simpl in H0); intuition; cset_tac.
+    edestruct (IHe1 F); eauto.
+    edestruct (IHe2 F); eauto.
+    rewrite H1, H4.
+    destruct if in H2; simpl in *; unfold val2bool in H2.
+   + erewrite bvEq_equiv_eq in H2.
+     rewrite e. unfold binop_eval.
+     unfold smt_eval in *; erewrite exp_eval_partial_total in H2; eauto.
+     unfold bvDiv. destruct if; isabsurd.
+     destruct (bvLessZero x); destruct (bvLessZero x0); eexists; eauto.
+   + unfold binop_eval; unfold option_lift2; simpl; case_eq b; intros; [ eexists; eauto |].
+     case_eq n0; intros; [ eexists; eauto | ].
+     case_eq n1; intros; [ eexists; eauto | ].
+     case_eq n2; intros; [ eexists; eauto | ].
+     case_eq n3; intros; [ eexists; eauto | ].
+     case_eq n4; intros; [ isabsurd | eexists; eauto].
 Qed.
 
-(* Not in thesis as simplified by guards = no option
--->approx Lemma 6**)
-Lemma noguardlist_impl_eval:
-  forall E el,
+(*  Lemma 6**)
+Lemma guardlist_impl_eval:
+  forall F E el,
     (forall x, x ∈ list_union (List.map Exp.freeVars el) -> exists v,  E x = Some v)
-    -> undefLift el = None
+    -> models F (to_total E) (undefLift el)
     -> exists v, omap (exp_eval E) el = Some v.
 
 Proof.
   intros.
-  general induction el; simpl; eauto.
-  - eapply (combine_keep_undef_list) in H0.
-    destruct H0.
-    case_eq (exp_eval E a); intros; simpl.
-    + simpl in H0.  exploit (IHel E); eauto.
-      Focus 2.  destruct X. rewrite H3. exists (v::x); eauto.
-      intros; eapply H. unfold list_union; simpl.
-      eapply list_union_start_swap. cset_tac.
-      right; eauto.
-    + pose proof (noguard_impl_eval E a).
-      destruct H3; eauto; isabsurd.
-      intros; eapply H. unfold list_union; simpl.
-      eapply list_union_start_swap; cset_tac.
-      left; right; eauto.
-Qed.
-
-(** Lemma 6 in the thesis **)
-Lemma guard_impl_eval:
-forall F E e g,
- undef e = Some g
--> models F (to_total E) g
--> (forall x, x ∈ Exp.freeVars e -> exists v, E x = Some v)
--> exists v, exp_eval E e = Some v.
-
-Proof.
-intros. general induction e; try isabsurd; simpl.
-- destruct u; simpl in H.
-  + destruct (IHe F E g H H0) as [v eval]; cset_tac; eauto.
-    rewrite eval. simpl. unfold option_lift1.
-    destruct(val2bool v); eauto.
- + destruct (IHe F E g H H0) as [v eval]; cset_tac; eauto.
-   rewrite eval; simpl; unfold option_lift1.
-   exists (neg v); eauto.
-- destructBin b; simpl in *.
-  + case_eq (undef e1); case_eq (undef e2); intros; simpl in *;
-    rewrite H2, H3 in H; inversion H.
-    * rewrite <- H5 in H0; simpl in H0.
-      destruct H0.
-      destruct (IHe1 F E s0 H3 H0); cset_tac; eauto.
-      destruct (IHe2 F E s H2 H4); cset_tac; eauto.
-      rewrite H6, H5; simpl. exists (bvAdd x x0); eauto.
-    *  pose proof (noguard_impl_eval E e2).
-       destruct H4; cset_tac; eauto.
-       destruct (IHe1 F E g); cset_tac; eauto.
-       rewrite H4, H5; simpl; unfold option_lift2.
-       exists (bvAdd x0 x); eauto.
-    * pose proof (noguard_impl_eval E e1).
-      destruct H4; cset_tac; eauto.
-      destruct (IHe2 F E g); cset_tac; eauto.
-      rewrite H4, H5. simpl. exists (bvAdd x x0); eauto.
-  + case_eq (undef e1); case_eq (undef e2); intros; simpl in *;
-    rewrite H2, H3 in H; inversion H.
-    * rewrite <- H5 in H0; simpl in H0.
-      destruct H0.
-      destruct (IHe1 F E s0 H3 H0); cset_tac; eauto.
-      destruct (IHe2 F E s H2 H4); cset_tac; eauto.
-      rewrite H6, H5; simpl. exists (bvSub x x0); eauto.
-    *  pose proof (noguard_impl_eval E e2 ).
-       destruct H4; cset_tac; eauto.
-       destruct (IHe1 F E g); cset_tac; eauto.
-       rewrite H4, H5; simpl; unfold option_lift2.
-       exists (bvSub x0 x); eauto.
-    * pose proof (noguard_impl_eval E e1).
-      destruct H4; cset_tac; eauto.
-      destruct (IHe2 F E g); cset_tac; eauto.
-      rewrite H4, H5. simpl. exists (bvSub x x0); eauto.
-  + case_eq (undef e1); case_eq (undef e2); intros; simpl in *;
-    rewrite H2, H3 in H; inversion H.
-    * rewrite <- H5 in H0; simpl in H0.
-      destruct H0.
-      destruct (IHe1 F E s0 H3 H0); cset_tac; eauto.
-      destruct (IHe2 F E s H2 H4); cset_tac; eauto.
-      rewrite H6, H5; simpl. exists (bvMult x x0); eauto.
-    *  pose proof (noguard_impl_eval E e2 ).
-       destruct H4; cset_tac; eauto.
-       destruct (IHe1 F E g); cset_tac; eauto.
-       rewrite H4, H5; simpl; unfold option_lift2.
-       exists (bvMult x0 x); eauto.
-    * pose proof (noguard_impl_eval E e1).
-      destruct H4; cset_tac; eauto.
-      destruct (IHe2 F E g); cset_tac; eauto.
-      rewrite H4, H5. simpl. exists (bvMult x x0); eauto.
-  + case_eq (undef e1); case_eq (undef e2); intros; simpl in *;
-    rewrite H2, H3 in H; inversion H.
-    * rewrite <- H5 in H0; simpl in H0.
-      destruct H0.
-      destruct (IHe1 F E s0 H3 H0); cset_tac; eauto.
-      destruct (IHe2 F E s H2 H4); cset_tac; eauto.
-      rewrite H6, H5; simpl. exists (bvEq x x0); eauto.
-    *  pose proof (noguard_impl_eval E e2 ).
-       destruct H4; cset_tac; eauto.
-       destruct (IHe1 F E g); cset_tac; eauto.
-       rewrite H4, H5; simpl; unfold option_lift2.
-       exists (bvEq x0 x); eauto.
-    * pose proof (noguard_impl_eval E e1).
-      destruct H4; cset_tac; eauto.
-      destruct (IHe2 F E g); cset_tac; eauto.
-      rewrite H4, H5. simpl. exists (bvEq x x0); eauto.
-  + case_eq (undef e1); case_eq (undef e2); intros; simpl in *;
-    rewrite H2, H3 in H; inversion H.
-    * rewrite <- H5 in H0; simpl in H0.
-      destruct H0.
-      destruct (IHe1 F E s0 H3 H0); cset_tac; eauto.
-      destruct (IHe2 F E s H2 H4); cset_tac; eauto.
-      rewrite H6, H5; simpl. exists (neg (bvEq x x0)); eauto.
-    *  pose proof (noguard_impl_eval E e2).
-       destruct H4; cset_tac; eauto.
-       destruct (IHe1 F E g); cset_tac; eauto.
-       rewrite H4, H5; simpl; unfold option_lift2.
-       exists (neg (bvEq x0 x)); eauto.
-    * pose proof (noguard_impl_eval E e1).
-      destruct H4; cset_tac; eauto.
-      destruct (IHe2 F E g); cset_tac; eauto.
-      rewrite H4, H5. simpl. exists (neg (bvEq x x0)); eauto.
-  + case_eq (undef e1); case_eq (undef e2); intros; simpl in *;
-    rewrite H2, H3 in H; simpl in H; inversion H.
-    rewrite <- H5 in H0.
-    * destruct H0.  clear H5. clear H. simpl in H0. simpl in H0.
-      destruct H4.
-      destruct (IHe1 F E s0); cset_tac; eauto.
-      destruct (IHe2  F E s); cset_tac; eauto.
-      rewrite H5, H6; simpl.
-      unfold smt_eval in H0;
-      erewrite exp_eval_partial_total in H0; eauto.
-      clear H5. clear H6. clear H1.
-      unfold bvDiv.
-      case_eq (bvZero x0); intros.
-      { eapply (zero_implies_eq x0) in H1. specialize (H0 H1); isabsurd.
-        unfold zext. simpl; eauto. }
-      { eauto. }
-    * rewrite <- H5 in H0.  destruct H0.
-      clear H5; clear H. simpl in H0. simpl in H0.
-      pose proof (noguard_impl_eval E e2).
-      destruct H; cset_tac; eauto.
-      destruct (IHe1 F E s); eauto.
-      rewrite H, H5; simpl.
-      unfold smt_eval in H0;
-      erewrite exp_eval_partial_total in H0; eauto.
-      clear H. clear H5. clear H1.
-      unfold bvDiv. simpl.
-      case_eq (bvZero x); intros.
-      { eapply (zero_implies_eq x (b:=(zext k (O::nil)))) in H.
-        simpl in H. specialize (H0 H); isabsurd.  f_equal; eauto. }
-      { eauto. }
-    * rewrite <- H5 in H0; destruct H0; clear H5; clear H.
-      simpl in H0. simpl in H0.
-      pose proof (noguard_impl_eval  E e1).
-      destruct H; cset_tac; eauto.
-      destruct (IHe2 F E s); eauto.
-      rewrite H, H5; simpl.
-      unfold smt_eval in H0;
-      erewrite exp_eval_partial_total in H0; eauto.
-      clear H. clear H5. clear H1.
-      unfold bvDiv.
-      case_eq (bvZero x0); intros.
-      { eapply (zero_implies_eq x0 (b:=(zext k (O::nil)))) in H.
-        simpl in H. specialize (H0 H); isabsurd.  f_equal; eauto. }
-      { eauto. }
-    * rewrite <- H5 in H0. clear H5. simpl in H0.
-      pose proof (noguard_impl_eval E e1).
-      pose proof (noguard_impl_eval E e2).
-      destruct H4; cset_tac;  eauto.
-      destruct H5; cset_tac; eauto.
-      rewrite H4, H5. simpl.
-      unfold smt_eval in H0;
-      erewrite exp_eval_partial_total in H0; eauto.
-      simpl in H0.
-      unfold bvDiv. case_eq (bvZero x0); intros; eauto.
-      eapply (zero_implies_eq x0 (b:=zext k (O::nil))) in H6.
-      specialize (H0 H6); isabsurd.
-      f_equal; eauto.
-Qed.
-
-(** Lifted version of Lemma 6 **)
-Lemma guardList_impl_eval :
-forall F E el g,
- undefLift el = Some g
--> models F (to_total E) g
--> (forall x, x ∈ list_union (List.map Exp.freeVars el) -> exists v, E x = Some v)
--> exists v, (omap (exp_eval E) el) = Some v.
-
-Proof.
-  intros.
-  general induction el; eauto.
-  pose proof (exp_freeVars_list_agree E a el H1).
-  destruct H2.
-  - simpl in *.
-    case_eq (undef a); case_eq (undefLift el); intros;
-    rewrite H4, H5 in *; simpl in *;
-    inversion H; subst; simpl in *; try destruct H0.
-    + destruct (guard_impl_eval F E a s0); eauto.
-      rewrite H7; simpl.
-      destruct (IHel F E s); eauto.
-      exists (x::x0); rewrite H8; simpl; eauto.
-    + destruct (guard_impl_eval F E a g); eauto.
-      rewrite H6; simpl.
-      destruct (noguardlist_impl_eval E el); eauto.
-      exists (x::x0); rewrite H7; simpl; eauto.
-    + destruct (noguard_impl_eval E a); eauto.
-      rewrite H6.
-      destruct (IHel F E g); eauto.
-      exists (x::x0); rewrite H7; simpl; eauto.
+  general induction el; simpl in *; eauto.
+  eapply models_combine in H0; simpl in H0.
+  destruct H0.
+  edestruct IHel; eauto.
+  - eapply exp_freeVars_list_agree; eauto.
+  - rewrite H2. edestruct guard_models_impl_eval; eauto.
+    + eapply exp_freeVars_list_agree; eauto.
+    + rewrite H3; eexists; simpl; eauto.
 Qed.
 
 (** Lemma 7 in thesis **)
 Lemma guardTrue_if_Terminates_ret:
-forall L L' E s E' e g,
+forall L L' E s E' e,
 noFun s
--> undef e = Some g
 -> Terminates (L, E, s)(L', E', stmtReturn e)
--> forall F, models F (to_total E') g.
+-> forall F, models F (to_total E') (undef e).
 
 Proof.
-intros. general induction H1.
-- eapply (guard_true_if_eval); eauto.
-- specialize (IHTerminates L0 L'0 E' s' E'0 e g).
-  inversion H2.
-  + rewrite <- H5 in *. inversion H; subst.
-    eapply IHTerminates; eauto.
-  + rewrite <- H6 in *; inversion H; subst.
-    * eapply IHTerminates; eauto.
-    * eapply IHTerminates; eauto.
-  + rewrite <- H4 in H0. exfalso; specialize (H0 l Y); isabsurd .
-  + rewrite <- H4 in *.  exfalso. inversion H.
+  intros. general induction H0; eauto using guard_true_if_eval.
+  specialize (IHTerminates L0 L'0 E' s' E'0 e).
+  inversion H; subst; invt noFun; eauto using IHTerminates; eauto.
+  isabsurd.
 Qed.
 
 Lemma guardTrue_if_Terminates_goto:
-forall L L' E s E' f x g,
+forall L L' E s E' f el,
 noFun s
--> undefLift x = Some g
--> Terminates (L, E, s) (L', E' , stmtGoto f x)
--> forall F, models F (to_total E') g.
+-> Terminates (L, E, s) (L', E' , stmtGoto f el)
+-> forall F, models F (to_total E') (undefLift el).
 
 Proof.
-intros. general induction H1.
-- eapply guardList_true_if_eval; eauto.
-- specialize (IHTerminates L0 L'0  E' s' E'0 f x g).
-  inversion H2.
-  + rewrite <- H5 in *. inversion H; subst.
-    eapply IHTerminates; eauto.
-  + rewrite <- H6 in *. inversion H; subst.
-    * eapply IHTerminates; eauto.
-    * eapply IHTerminates; eauto.
-  + rewrite <- H4 in *; specialize (H0 l Y); isabsurd.
-  + rewrite <- H4 in *; inversion H.
+  intros. general induction H0; eauto using guardList_true_if_eval.
+  specialize (IHTerminates L0 L'0  E' s' E'0 f el).
+  inversion H; subst; invt noFun; eauto using IHTerminates; eauto.
+  isabsurd.
 Qed.
 
 (** Lemma 9 in the Thesis **)
 Lemma undef_models:
-forall F E e g,
+forall F E e,
 (forall x, x ∈ Exp.freeVars e -> exists v, E x = Some v)
--> undef e =Some g
 -> exp_eval E e = None
--> ~ models F (to_total E) g.
+-> ~ models F (to_total E) (undef e).
 
 Proof.
-intros;  hnf;  intros.
-general induction e; simpl in *; try isabsurd.
-- monad_inv H1.
-  + specialize (IHe F E g H H0 H3 H2); eauto.
-  + destruct u; isabsurd.
-- destructBin b; monad_inv H1; try isabsurd.
-  + case_eq (undef e1); case_eq (undef e2); intros;
-    rewrite H4 in H0; rewrite H1 in H0; simpl in H0; inversion H0;
-    rewrite <- H6 in H2; simpl in H2; try destruct H2.
-    * eapply (IHe1 F E s0); eauto.
-      intros. cset_tac. specialize (H x). destruct H; eauto.
-    * eapply (IHe1 F E s); eauto.
-      intros; cset_tac; specialize (H x); destruct H; eauto.
-    * pose proof (noguard_impl_eval  E e1).
-      destruct H5; isabsurd; eauto.
-      intros; cset_tac; destruct (H x); eauto.
-  + case_eq (undef e1); case_eq (undef e2); intros;
-    rewrite H4 in H0; rewrite H3 in H0; simpl in H0; inversion H0;
-    rewrite <- H6 in H2; simpl in H2; try destruct H2.
-    * eapply (IHe2 F E s); eauto.
-      intros; cset_tac. destruct (H x0); eauto.
-    * pose proof (noguard_impl_eval E e2).
-      destruct H5; isabsurd; eauto.
-      intros; cset_tac. destruct (H x0); eauto.
-    * eapply (IHe2 F E s); eauto.
-      intros; cset_tac. destruct (H x0); eauto.
-  +  case_eq (undef e1); case_eq (undef e2); intros;
-    rewrite H4 in H0; rewrite H1 in H0; simpl in H0; inversion H0;
-    rewrite <- H6 in H2; simpl in H2; try destruct H2.
-     * eapply (IHe1 F E s0); eauto.
-       intros; cset_tac. destruct (H x); eauto.
-     * eapply (IHe1 F E s); eauto.
-       intros; cset_tac; destruct (H x); eauto.
-     * pose proof (noguard_impl_eval E e1).
-       destruct H5; eauto; isabsurd.
-       intros; cset_tac; destruct (H x); eauto.
-  + case_eq (undef e1); case_eq (undef e2); intros;
-    rewrite H4 in H0; rewrite H3 in H0; simpl in H0; inversion H0;
-    rewrite <- H6 in H2; simpl in H2; try destruct H2.
-    * eapply (IHe2 F E s); eauto.
-      intros; cset_tac. destruct (H x0); eauto.
-    * pose proof (noguard_impl_eval E e2).
-      destruct H5; eauto; isabsurd.
-      intros; cset_tac. destruct (H x0); eauto.
-    * eapply (IHe2 F E s); eauto.
-      intros; cset_tac. destruct (H x0); eauto.
-  + case_eq (undef e1); case_eq (undef e2); intros;
-    rewrite H4 in H0; rewrite H1 in H0; simpl in H0; inversion H0;
-    rewrite <- H6 in H2; simpl in H2; try destruct H2.
-     * eapply (IHe1 F E s0); eauto.
-       intros; cset_tac. destruct (H x); eauto.
-     * eapply (IHe1 F E s); eauto.
-       intros; cset_tac; destruct (H x); eauto.
-     * pose proof (noguard_impl_eval  E e1).
-       destruct H5; eauto; isabsurd.
-       intros; cset_tac; destruct (H x); eauto.
-  + case_eq (undef e1); case_eq (undef e2); intros;
-    rewrite H4 in H0; rewrite H3 in H0; simpl in H0; inversion H0;
-    rewrite <- H6 in H2; simpl in H2; try destruct H2.
-    * eapply (IHe2 F E s); eauto.
-      intros; cset_tac. destruct (H x0); eauto.
-    * pose proof (noguard_impl_eval E e2).
-      destruct H5; eauto; isabsurd.
-      intros; cset_tac. destruct (H x0); eauto.
-    * eapply (IHe2 F E s); eauto.
-      intros; cset_tac. destruct (H x0); eauto.
-  + case_eq (undef e1); case_eq (undef e2); intros;
-    rewrite H4 in H0; rewrite H1 in H0; simpl in H0; inversion H0;
-    rewrite <- H6 in H2; simpl in H2; try destruct H2.
-     * eapply (IHe1 F E s0); eauto.
-       intros; cset_tac. destruct (H x); eauto.
-     * eapply (IHe1 F E s); eauto.
-       intros; cset_tac; destruct (H x); eauto.
-     * pose proof (noguard_impl_eval E e1).
-       destruct H5; eauto; isabsurd.
-       intros; cset_tac; destruct (H x); eauto.
-  +  case_eq (undef e1); case_eq (undef e2); intros;
-    rewrite H4 in H0; rewrite H3 in H0; simpl in H0; inversion H0;
-    rewrite <- H6 in H2; simpl in H2; try destruct H2.
-     * eapply (IHe2 F E s); eauto.
-       intros; cset_tac. destruct (H x0); eauto.
-     * pose proof (noguard_impl_eval E e2).
-       destruct H5; eauto; isabsurd.
-       intros; cset_tac. destruct (H x0); eauto.
-     * eapply (IHe2 F E s); eauto.
-       intros; cset_tac. destruct (H x0); eauto.
-  + case_eq (undef e1); case_eq (undef e2); intros;
-    rewrite H4 in H0; rewrite H1 in H0; simpl in H0; inversion H0;
-    rewrite <- H6 in H2; simpl in H2; try destruct H2.
-    * eapply (IHe1 F E s0); eauto.
-      intros; cset_tac. destruct (H x); eauto.
-    * eapply (IHe1 F E s); eauto.
-      intros; cset_tac; destruct (H x); eauto.
-    * pose proof (noguard_impl_eval E e1).
-      destruct H5; eauto; isabsurd.
-      intros; cset_tac; destruct (H x); eauto.
-  +  case_eq (undef e1); case_eq (undef e2); intros;
-    rewrite H4 in H0; rewrite H3 in H0; simpl in H0; inversion H0;
-    rewrite <- H6 in H2; simpl in H2; try destruct H2.
-     * eapply (IHe2 F E s); eauto.
-       intros; cset_tac. destruct (H x0); eauto.
-     * pose proof (noguard_impl_eval E e2).
-       destruct H5; eauto; isabsurd.
-       intros; cset_tac. destruct (H x0); eauto.
-     * eapply (IHe2 F E s); eauto.
-       intros; cset_tac. destruct (H x0); eauto.
-  + case_eq (undef e1); case_eq (undef e2); intros;
-    rewrite H1, H4 in H0; simpl in H0; inversion H0; clear H0;
-    rewrite <- H6 in H2; clear H6;
-    simpl in H2.
-    * destruct H2; destruct H2.  eapply (IHe1 F E s0); eauto.
-      intros; cset_tac. destruct (H x); eauto.
-    * destruct H2.  eapply (IHe1 F E s); eauto.
-      intros; cset_tac. destruct (H x); eauto.
-    * destruct H2. pose proof (noguard_impl_eval E e1); eauto.
-      destruct H5; eauto; isabsurd.
-      intros; cset_tac. destruct (H x); eauto.
-    * pose proof (noguard_impl_eval E e1).
-      destruct H0; eauto; isabsurd.
-      intros; cset_tac. destruct (H x); eauto.
-  +  case_eq (undef e1); case_eq (undef e2); intros;
-    rewrite H3, H4 in H0; simpl in H0; inversion H0; clear H0;
-    rewrite <- H6 in H2; clear H6;
-    simpl in H2; destruct H2; try destruct H2.
-     * eapply (IHe2 F E s); eauto.
-       intros; cset_tac. destruct (H x0); eauto.
-     * pose proof (noguard_impl_eval E e2).
-       destruct H5; eauto; isabsurd.
-       intros; cset_tac. destruct (H x0); eauto.
-     * eapply (IHe2 F E s); eauto.
-       intros; cset_tac. destruct (H x0); eauto.
-     * pose proof (noguard_impl_eval E e2).
-       destruct H0; eauto; isabsurd.
-       intros; cset_tac. destruct (H x0); eauto.
-  + case_eq (undef e1); case_eq (undef e2); intros;
-    rewrite H1, H3 in H0; simpl in H; inversion H0; clear H0;
-    rewrite <- H5 in H2; destruct H2; try destruct H2; clear H5.
-    * simpl in H1. destruct H1. simpl in EQ2. unfold bvDiv in EQ2.
-      apply H0.  case_eq(bvZero x0); intros.
-      Focus 2. rewrite H1 in EQ2. destruct (bvLessZero x); destruct (bvLessZero x0); isabsurd.
-      unfold smt_eval;
-      erewrite exp_eval_partial_total; eauto.
-      simpl.
-      change (val2bool (bvEq x0 (zext k (O::nil)))). clear H.  eapply zero_implies_eq; eauto.
-    * simpl in H1. destruct H1. simpl in EQ2. unfold bvDiv in EQ2.
-      apply H0.  case_eq(bvZero x0); intros.
-      Focus 2. rewrite H1 in EQ2. destruct (bvLessZero x); destruct (bvLessZero x0); isabsurd.
-      unfold smt_eval;
-      erewrite exp_eval_partial_total; eauto.
-      change (val2bool (bvEq x0 (zext k (O::nil)))). clear H.  eapply zero_implies_eq; eauto.
-    * simpl in H1. destruct H1. simpl in EQ2. unfold bvDiv in EQ2.
-      apply H0.  case_eq(bvZero x0); intros.
-      Focus 2. rewrite H1 in EQ2. destruct (bvLessZero x); destruct (bvLessZero x0); isabsurd.
-      unfold smt_eval;
-      erewrite exp_eval_partial_total; eauto.
-      change (val2bool (bvEq x0 (zext k (O::nil)))). clear H.  eapply zero_implies_eq; eauto.
-    * simpl in H1. destruct H1. simpl in EQ2. unfold bvDiv in EQ2.
-      case_eq(bvZero x0); intros.
-      Focus 2. rewrite H0 in EQ2. destruct (bvLessZero x); destruct (bvLessZero x0); isabsurd.
-      unfold smt_eval;
-      erewrite exp_eval_partial_total; eauto.
-      change (val2bool (bvEq x0 (zext k (O::nil)))).  eapply zero_implies_eq; eauto.
+  intros;  hnf;  intros.
+  general induction e; simpl in *; try isabsurd.
+  - specialize (H v); destruct H; cset_tac; eauto; isabsurd.
+  - monad_inv H0.
+    + eapply IHe; eauto.
+    + destruct u; isabsurd.
+  - repeat (rewrite models_combine in H1; simpl in H1).
+    destruct H1 as [[H1 H2] H3].
+    edestruct guard_models_impl_eval; eauto.
+    + eapply exp_freeVars_bin_agree; eauto.
+    + edestruct (guard_models_impl_eval F E e1); eauto.
+      * eapply (exp_freeVars_bin_agree E e1 e2); eauto.
+      *  unfold smt_eval.  rewrite H4, H5 in *; simpl in *.
+         destruct if in H3; simpl in H3.
+         { eapply H3. unfold val2bool; eapply bvEq_equiv_eq.
+           subst; simpl in *.
+           unfold smt_eval; erewrite exp_eval_partial_total; eauto.
+           unfold bvDiv in H0; destruct if in H0; subst; eauto; isabsurd. }
+         { destructBin b; subst; isabsurd. }
 Qed.
 
 (*
